code/ecdsap256/Hacl.Impl.P256.Finv.fsti
@@ -1,4 +1,4 @@
-module Hacl.Impl.P256.Finv // before: Hacl.Impl.P256.MM.Exponent
+module Hacl.Impl.P256.Finv
 
 open FStar.Mul
 open FStar.HyperStack.All
@@ -7,7 +7,6 @@ module ST = FStar.HyperStack.ST
 
 open Lib.IntTypes
 open Lib.Buffer
-
 
 open Spec.P256
 open Spec.P256.Constants
@@ -18,18 +17,18 @@ open Hacl.Spec.P256.Felem
 
 #set-options "--z3rlimit 30 --fuel 0 --ifuel 0"
 
-val exponent: a:felem -> result:felem -> tempBuffer:lbuffer uint64 (size 20) -> Stack unit
+val finv: a:felem -> res:felem -> tmp:lbuffer uint64 (size 20) -> Stack unit
   (requires fun h ->
-    live h a /\ live h tempBuffer /\ live h result /\
-    disjoint tempBuffer result /\ disjoint a tempBuffer /\
+    live h a /\ live h tmp /\ live h res /\
+    disjoint tmp res /\ disjoint a tmp /\
     as_nat h a < prime256)
-  (ensures fun h0 _ h1 -> modifies (loc result |+| loc tempBuffer) h0 h1 /\
-    as_nat h1 result = toDomain_ ((pow (fromDomain_ (as_nat h0 a)) (prime256 - 2)) % prime256))
+  (ensures fun h0 _ h1 -> modifies (loc res |+| loc tmp) h0 h1 /\
+    as_nat h1 res = toDomain_ ((pow (fromDomain_ (as_nat h0 a)) (prime256 - 2)) % prime256))
 
 
-val square_root: a:felem -> result:felem -> Stack unit
-  (requires fun h -> live h a /\ live h result /\ as_nat h a < prime)
-  (ensures fun h0 _ h1 -> modifies (loc a |+| loc result) h0 h1 /\
-    as_nat h1 result < prime /\
-    fromDomain_ (as_nat h1 result) = sq_root_spec (fromDomain_ (as_nat h0 a)) /\
-    fromDomain_ (as_nat h1 result) = pow (fromDomain_ (as_nat h0 a)) ((prime256 + 1) / 4) % prime256)
+val fsqrt: a:felem -> res:felem -> Stack unit
+  (requires fun h -> live h a /\ live h res /\ as_nat h a < prime)
+  (ensures fun h0 _ h1 -> modifies (loc a |+| loc res) h0 h1 /\
+    as_nat h1 res < prime /\
+    fromDomain_ (as_nat h1 res) = sq_root_spec (fromDomain_ (as_nat h0 a)) /\
+    fromDomain_ (as_nat h1 res) = pow (fromDomain_ (as_nat h0 a)) ((prime256 + 1) / 4) % prime256)
